LeanBF/Core.lean
@@ -6,6 +6,7 @@ Authors: Bangyen Pham
 import LeanBF.Core.Compiler
 import LeanBF.Core.Instruction
 import LeanBF.Core.Minsky
+import LeanBF.Core.Parser
 import LeanBF.Core.Semantics
 import LeanBF.Core.State
 
